Sequences/NatSeqConversions.dfy
@@ -1,18 +1,22 @@
 include "NatSeq.dfy"
+// TODO: Add examples of how these modules are used with assert statements
+// TODO: Add instantiation with common bounds - 8, 16, 32
+
+include "NatSeq.dfy"
 
 abstract module NatSeqConversions refines NatSeq {
 
-  import SmallBound
-  import LargeBound
+  import Small
+  import Large
 
-  /* SmallBound.BOUND() to the power of E() is LargeBound.BOUND(). */
+  /* Small.BOUND() to the power of E() is Large.BOUND(). */
   function method E(): nat
-    ensures power(SmallBound.BOUND(), E()) == LargeBound.BOUND()
+    ensures power(Small.BOUND(), E()) == Large.BOUND()
   {
     lemma_div_basics_auto();
     lemma_power_multiplies_auto();
-    lemma_fundamental_div_mod(LargeBound.BITS(), SmallBound.BITS());
-    LargeBound.BITS() / SmallBound.BITS()
+    lemma_fundamental_div_mod(Large.BITS(), Small.BITS());
+    Large.BITS() / Small.BITS()
   }
 
   lemma lemma_mod_eq_zero(x: nat, y: nat)
@@ -28,18 +32,18 @@ abstract module NatSeqConversions refines NatSeq {
     }
   }
 
-  /* Converts a sequence from LargeBound.BOUND() to SmallBound.BOUND(). */
-  function method {:opaque} to_smaller_bound(xs: seq<LargeBound.uint>): (ys: seq<SmallBound.uint>)
+  /* Converts a sequence from Large.BOUND() to Small.BOUND(). */
+  function method {:opaque} to_small(xs: seq<Large.uint>): (ys: seq<Small.uint>)
     ensures |ys| == |xs| * E()
   {
     if |xs| == 0 then []
     else
       lemma_mul_is_distributive_add_other_way(E(), 1, |xs| - 1);
-      SmallBound.from_nat_with_len(first(xs), E()) + to_smaller_bound(drop_first(xs))
+      Small.from_nat_with_len(first(xs), E()) + to_small(drop_first(xs))
   }
 
-  /* Converts a sequence from SmallBound.BOUND() to LargeBound.BOUND(). */
-  function method {:opaque} to_larger_bound(xs: seq<SmallBound.uint>): (ys: seq<LargeBound.uint>)
+  /* Converts a sequence from Small.BOUND() to Large.BOUND(). */
+  function method {:opaque} to_large(xs: seq<Small.uint>): (ys: seq<Large.uint>)
     requires |xs| % E() == 0
     ensures |ys| == |xs| / E()
   {
@@ -48,89 +52,129 @@ abstract module NatSeqConversions refines NatSeq {
       lemma_mod_eq_zero(|xs|, E());
       assert |xs| >= E();
 
-      SmallBound.lemma_seq_nat_bound(xs[..E()]);
+      Small.lemma_seq_nat_bound(xs[..E()]);
       lemma_mod_sub_multiples_vanish_auto();
       lemma_div_minus_one(|xs|, E());
-      [SmallBound.to_nat(xs[..E()]) as LargeBound.uint] + to_larger_bound(xs[E()..])
+      [Small.to_nat(xs[..E()]) as Large.uint] + to_large(xs[E()..])
   }
 
-  /* Sequence conversion from LargeBound.BOUND() to SmallBound.BOUND() does not
+  /* Sequence conversion from Large.BOUND() to Small.BOUND() does not
   change its nat representation. */
-  lemma lemma_smaller_bound_to_nat(xs: seq<LargeBound.uint>)
-    ensures SmallBound.to_nat(to_smaller_bound(xs)) == LargeBound.to_nat(xs)
+  lemma lemma_to_small(xs: seq<Large.uint>)
+    ensures Small.to_nat(to_small(xs)) == Large.to_nat(xs)
   {
-    reveal LargeBound.to_nat();
-    reveal SmallBound.to_nat();
-    reveal to_smaller_bound();
+    reveal Large.to_nat();
+    reveal Small.to_nat();
+    reveal to_small();
     if |xs| > 0 {
       calc {
-        SmallBound.to_nat(to_smaller_bound(xs));
-        SmallBound.to_nat(SmallBound.from_nat_with_len(first(xs), E()) + to_smaller_bound(drop_first(xs)));
-          { SmallBound.lemma_seq_prefix(SmallBound.from_nat_with_len(first(xs), E()) + to_smaller_bound(drop_first(xs)), E()); }
-        SmallBound.to_nat(SmallBound.from_nat_with_len(first(xs), E())) + SmallBound.to_nat(to_smaller_bound(drop_first(xs))) * power(SmallBound.BOUND(), E());
+        Small.to_nat(to_small(xs));
+        Small.to_nat(Small.from_nat_with_len(first(xs), E()) + to_small(drop_first(xs)));
           {
-            SmallBound.lemma_from_nat_with_len_eq_from_nat(first(xs), E());
-            SmallBound.lemma_nat_seq_nat(first(xs));
-            lemma_smaller_bound_to_nat(drop_first(xs));
+            Small.lemma_seq_prefix(Small.from_nat_with_len(first(xs), E()) + to_small(drop_first(xs)), E());
+            lemma_to_small(drop_first(xs));
           }
-        first(xs) + LargeBound.to_nat(drop_first(xs)) * power(SmallBound.BOUND(), E());
-          { assert power(SmallBound.BOUND(), E()) == LargeBound.BOUND(); }
-        LargeBound.to_nat(xs);
+        first(xs) + Large.to_nat(drop_first(xs)) * power(Small.BOUND(), E());
+          { assert power(Small.BOUND(), E()) == Large.BOUND(); }
+        Large.to_nat(xs);
       }
     }
   }
 
-  /* Sequence conversion from SmallBound.BOUND() to LargeBound.BOUND() does not
+  /* Sequence conversion from Small.BOUND() to Large.BOUND() does not
   change its nat representation. */
-  lemma lemma_larger_bound_to_nat(xs: seq<SmallBound.uint>)
+  lemma lemma_to_large(xs: seq<Small.uint>)
     requires |xs| % E() == 0
-    ensures LargeBound.to_nat(to_larger_bound(xs)) == SmallBound.to_nat(xs)
+    ensures Large.to_nat(to_large(xs)) == Small.to_nat(xs)
   {
-    reveal LargeBound.to_nat();
-    reveal SmallBound.to_nat();
-    reveal to_larger_bound();
+    reveal Large.to_nat();
+    reveal Small.to_nat();
+    reveal to_large();
     if |xs| > 0 {
       calc {
-        LargeBound.to_nat(to_larger_bound(xs));
+        Large.to_nat(to_large(xs));
           {
             lemma_mod_eq_zero(|xs|, E());
             lemma_mod_sub_multiples_vanish_auto();
-            SmallBound.lemma_seq_nat_bound(xs[..E()]);
+            Small.lemma_seq_nat_bound(xs[..E()]);
           }
-        LargeBound.to_nat([SmallBound.to_nat(xs[..E()]) as LargeBound.uint] + to_larger_bound(xs[E()..]));
-          { lemma_larger_bound_to_nat(xs[E()..]); }
-        SmallBound.to_nat(xs[..E()]) + SmallBound.to_nat(xs[E()..]) * power(SmallBound.BOUND(), E());
-          { SmallBound.lemma_seq_prefix(xs, E()); }
-        SmallBound.to_nat(xs);
+        Large.to_nat([Small.to_nat(xs[..E()]) as Large.uint] + to_large(xs[E()..]));
+          { lemma_to_large(xs[E()..]); }
+        Small.to_nat(xs[..E()]) + Small.to_nat(xs[E()..]) * power(Small.BOUND(), E());
+          { Small.lemma_seq_prefix(xs, E()); }
+        Small.to_nat(xs);
       }
     }
   }
 
-  /* to_smaller_bound is injective. */
-  lemma lemma_to_smaller_bound_is_injective(xs: seq<LargeBound.uint>,
-                                            ys: seq<LargeBound.uint>)
-    requires to_smaller_bound(xs) == to_smaller_bound(ys)
+  /* to_small is injective. */
+  lemma lemma_to_small_is_injective(xs: seq<Large.uint>, ys: seq<Large.uint>)
+    requires to_small(xs) == to_small(ys)
     requires |xs| == |ys|
     ensures xs == ys
   {
-    lemma_smaller_bound_to_nat(xs);
-    lemma_smaller_bound_to_nat(ys);
-    assert LargeBound.to_nat(xs) == LargeBound.to_nat(ys);
-    LargeBound.lemma_seq_eq(xs, ys);
+    lemma_to_small(xs);
+    lemma_to_small(ys);
+    assert Large.to_nat(xs) == Large.to_nat(ys);
+    Large.lemma_seq_eq(xs, ys);
   }
 
-  /* to_larger_bound is injective. */
-  lemma lemma_to_larger_bound_is_injective(xs: seq<SmallBound.uint>,
-                                           ys: seq<SmallBound.uint>)
+  /* to_large is injective. */
+  lemma lemma_to_large_is_injective(xs: seq<Small.uint>, ys: seq<Small.uint>)
     requires |xs| % E() == |ys| % E() == 0 
-    requires to_larger_bound(xs) == to_larger_bound(ys)
+    requires to_large(xs) == to_large(ys)
     requires |xs| == |ys|
     ensures xs == ys
   {
-    lemma_larger_bound_to_nat(xs);
-    lemma_larger_bound_to_nat(ys);
-    assert SmallBound.to_nat(xs) == SmallBound.to_nat(ys);
-    SmallBound.lemma_seq_eq(xs, ys);
+    lemma_to_large(xs);
+    lemma_to_large(ys);
+    assert Small.to_nat(xs) == Small.to_nat(ys);
+    Small.lemma_seq_eq(xs, ys);
+  }
+
+  lemma lemma_small_large_small(xs: seq<Small.uint>)
+    requires |xs| % E() == 0
+    ensures to_small(to_large(xs)) == xs
+  {
+    reveal to_small();
+    reveal to_large();
+    if |xs| > 0 {
+      calc {
+        to_small(to_large(xs));
+          {
+            lemma_mod_eq_zero(|xs|, E());
+            Small.lemma_seq_nat_bound(xs[..E()]);
+            lemma_mod_sub_multiples_vanish_auto();
+          }
+        to_small([Small.to_nat(xs[..E()]) as Large.uint] + to_large(xs[E()..]));
+        Small.from_nat_with_len(Small.to_nat(xs[..E()]), E()) + to_small(to_large(xs[E()..]));
+          {
+            Small.lemma_seq_nat_seq(xs[..E()]);
+            lemma_small_large_small(xs[E()..]);
+          }
+        xs;
+      }
+    }
+  }
+
+  lemma lemma_large_small_large(xs: seq<Large.uint>)
+    ensures |to_small(xs)| % E() == 0
+    ensures to_large(to_small(xs)) == xs
+  {
+    reveal to_small();
+    reveal to_large();
+    lemma_mod_multiples_basic_auto();
+    if |xs| > 0 {
+      calc {
+        to_large(to_small(xs));
+        to_large(Small.from_nat_with_len(first(xs), E()) + to_small(drop_first(xs)));
+        [Small.to_nat(Small.from_nat_with_len(first(xs), E())) as Large.uint] + to_large(to_small(drop_first(xs)));
+        [first(xs)] + to_large(to_small(drop_first(xs)));
+          { lemma_large_small_large(drop_first(xs)); }
+        [first(xs)] + drop_first(xs);
+        xs;
+      }
+    }
   }
 
 }
